

1) Single Output, single sample

$$\hat{y} = w^T x + b, L = (\hat{y} - y)^2$$

$$\frac{dL}{dw} = \frac{dL}{d\hat{y}} \cdot \frac{d\hat{y}}{dw} = 2(\hat{y} - y)x$$

$$\frac{dL}{db} = \frac{dL}{d\hat{y}} \cdot \frac{d\hat{y}}{db} = 2(\hat{y} - y)$$

2) Single Output, Many Samples, N samples

$$\text{MSE : } L = \frac{1}{N} \sum_{i=1}^N (\hat{y}_i - y_i)^2$$

$$\frac{dL}{dw} = \frac{d}{dw} \left(\frac{1}{N} \sum_{i=1}^N (\hat{y}_i - y_i)^2 \right) = \frac{1}{N} \sum_{i=1}^N \frac{d}{dw} (\hat{y}_i - y_i)^2 = \frac{1}{N} \sum_{i=1}^N 2(\hat{y}_i - y_i)x_i$$

$$= \frac{2}{N} \sum_{i=1}^N (\hat{y}_i - y_i)x_i$$

$$\frac{dL}{db} = \frac{2}{N} \sum_{i=1}^N (\hat{y}_i - y_i)$$

3) Many Outputs

N : # of samples
 M : # of input features
 D : # of outputs

$X_{N,M}$ $W_{M,D}$ $\hat{y}_{N,D}$

For a sample i and output j , $\hat{y}_{i,j} = \sum_{k=1}^M X_{i,k} W_{k,j} + b_j$

$$\text{MSE: } L = \frac{1}{N} \sum_{i=1}^N \sum_{j=1}^D (\hat{y}_{i,j} - y_{i,j})^2$$

$$\frac{dL}{dW_{k,j}} = \frac{d}{dW_{k,j}} \left(\frac{1}{N} \sum_{i=1}^N \sum_{j=1}^D (\hat{y}_{i,j} - y_{i,j})^2 \right) = \frac{1}{N} \sum_{i=1}^N \frac{d}{dW_{k,j}} (\hat{y}_{i,j} - y_{i,j})^2$$

$$\frac{d}{dW_{k,j}} (\hat{y}_{i,j} - y_{i,j})^2 = 2(\hat{y}_{i,j} - y_{i,j}) \frac{d\hat{y}_{i,j}}{dW_{k,j}} = 2(\hat{y}_{i,j} - y_{i,j}) X_{i,k}$$

$$\frac{dL}{dW_{k,j}} = \frac{1}{N} \sum_{i=1}^N 2(\hat{y}_{i,j} - y_{i,j}) X_{i,k} = 2/N \sum_{i=1}^N (\hat{y}_{i,j} - y_{i,j}) X_{i,k}$$

$$\frac{dL}{dW} = 2/N X^T (\hat{y} - y)$$

$(M \times D)$ $(M \times N)$ $(N \times D)$ $(N \times D)$

$$\frac{dL}{db_j} = \frac{1}{N} \sum_{i=1}^N 2(\hat{y}_{i,j} - y_{i,j}) \cdot \frac{dy_{i,j}}{db_j} = \frac{2}{N} \sum_{i=1}^N (\hat{y}_{i,j} - y_{i,j})$$

$(N \times D)$

$$\frac{dL}{db} = \frac{2}{N} \text{ALL-ONES} * (\hat{y} - y)$$

$(1 \times N)$ $(N \times D)$
 $\mathbf{1}_{1 \times N}$